util/vfmTypesScript.sml
@@ -1,6 +1,6 @@
 Theory vfmTypes
 Ancestors
-  byte list combin numposrep words
+  arithmetic byte list rich_list combin numposrep words
   keccak
 Libs
   blastLib
@@ -228,4 +228,50 @@ Proof
   \\ fs[Abbr`ls`]
   \\ irule l2n_n2l
   \\ rw[]
+QED
+
+Definition take_pad_0_def:
+  take_pad_0 z l = PAD_RIGHT 0w z (TAKE z l)
+End
+
+Theorem take_pad_0_0[simp]:
+  take_pad_0 0 l = []
+Proof
+  rw[take_pad_0_def, PAD_RIGHT]
+QED
+
+Theorem LENGTH_take_pad_0[simp]:
+  LENGTH (take_pad_0 z l) = z
+Proof
+  rw[take_pad_0_def, bitstringTheory.length_pad_right, LENGTH_TAKE_EQ]
+QED
+
+Theorem take_pad_0_IS_PREFIX:
+  ∃m. take_pad_0 n t ≼ t ++ REPLICATE m 0w
+Proof
+  rw[take_pad_0_def, PAD_RIGHT, IS_PREFIX_APPEND]
+  \\ `t = TAKE n t ++ DROP n t` by simp[]
+  \\ pop_assum(fn th => CONV_TAC(STRIP_QUANT_CONV(LAND_CONV(ONCE_REWRITE_CONV[th]))))
+  \\ simp[REPLICATE_GENLIST, LENGTH_TAKE_EQ]
+  \\ rw[DROP_LENGTH_TOO_LONG]
+  \\ qexists_tac`n - LENGTH t` \\ rw[]
+QED
+
+Theorem PAD_RIGHT_CONS:
+  PAD_RIGHT x y (h::t) = h::PAD_RIGHT x (PRE y) t
+Proof
+  rw[PAD_RIGHT] \\ Cases_on`y` \\ gs[]
+QED
+
+(* alternative characterisation *)
+Theorem take_pad_0_pad_take:
+  take_pad_0 z l = TAKE z (PAD_RIGHT 0w z l)
+Proof
+  rw[take_pad_0_def]
+  \\ qid_spec_tac`z`
+  \\ Induct_on`l`
+  \\ gs[bitstringTheory.length_pad_right]
+  \\ rw[Once TAKE_def]
+  >- EVAL_TAC
+  \\ gs[PAD_RIGHT_CONS, PRE_SUB1]
 QED
