prog/vfmProgScript.sml
@@ -493,36 +493,6 @@ Proof
   \\ metis_tac[]
 QED
 
-(* TODO: move *)
-Theorem FLOOKUP_parse_code_SOME_less_LENGTH:
-  ∀pc fm code x i.
-    FLOOKUP (parse_code pc fm code) x = SOME i ⇒
-    x ∈ FDOM fm ∨ x < pc + LENGTH code
-Proof
-  ho_match_mp_tac parse_code_ind
-  \\ rpt gen_tac \\ strip_tac
-  \\ rpt gen_tac \\ strip_tac
-  \\ Cases_on`NULL code` \\ gvs[NULL_EQ]
-  >- gvs[Once parse_code_def, TO_FLOOKUP]
-  \\ qhdtm_x_assum`FLOOKUP`mp_tac
-  \\ rw[Once parse_code_def, NULL_EQ]
-  \\ first_x_assum drule
-  \\ strip_tac \\ gvs[]
-  \\ gvs[NULL_EQ, FLOOKUP_UPDATE]
-  >- (Cases_on`code` \\ gs[])
-  \\ qmatch_asmsub_abbrev_tac`pc + l`
-  \\ Cases_on`l < LENGTH code` \\ gvs[]
-  \\ Cases_on`parse_opcode code`  \\ gvs[]
-  >- (gvs[vfmOperationTheory.opcode_def,Abbr`l`]
-      \\ Cases_on`code` \\ gvs[])
-  \\ gvs[DROP_LENGTH_TOO_LONG]
-  \\ gs[Once parse_code_def]
-  \\ gs[FLOOKUP_UPDATE]
-  \\ Cases_on`pc = x` \\ gvs[]
-  >- (Cases_on`code` \\ gs[])
-  \\ gs[TO_FLOOKUP]
-QED
-
 Theorem FLOOKUP_parse_code_0[local,simp]:
   FLOOKUP (parse_code 0 FEMPTY code) pc = SOME i ⇒
   ¬(LENGTH code ≤ pc)
